proof/invariant-abstract/Invariants_AI.thy
@@ -268,9 +268,6 @@ where
   (if f < 2^n  then {p+of_nat f .. p + 2 ^ n - 1} else {})"
 
 definition
-  "obj_range p obj \<equiv> {p .. p + 2^obj_bits obj - 1}" (* FIXME mask_range *)
-
-definition
   "pspace_no_overlap S \<equiv>
            \<lambda>s. \<forall>x ko. kheap s x = Some ko \<longrightarrow>
                 {x .. x + (2 ^ obj_bits ko - 1)} \<inter> S = {}" (* FIXME obj_range *)
